proxy/AppType.v
@@ -1,0 +1,14 @@
+From HTTP2.src Require Import Types HPACK.HPACKAbs.
+From HTTP2.src.Util Require Import OptionE.
+From Coq Require Import String.
+Require Import ExtLib.Data.Monads.StateMonad.
+
+Module Type AppType (codec:HPACK).
+  Parameter app_state : Type.
+  Parameter init : app_state -> app_state.
+  Parameter init_app_state : app_state.
+
+  Definition APP := state app_state.
+
+  Parameter execute : string -> APP (optionE string).
+End AppType.
