proxy/GenericServerType.v
@@ -1,0 +1,11 @@
+Require Import HTTP2.proxy.AppType.
+From ExtLib Require Export StateMonad.
+From Coq Require Export String.
+
+Module Type GenericServerType (app : AppType).
+  Parameter server_state: Type.
+  Parameter init_server_state: server_state.
+  Definition SERVER := stateT server_state app.APP.
+  
+  Parameter execute: (nat * string) -> SERVER (list (nat * string)).
+End GenericServerType.
