src/Decode.v
@@ -1,4 +1,4 @@
-From HTTP2 Require Import
+From HTTP2.src Require Import
      Equiv
      Types
      Util.BitVector
