src/HPACK/HPACKAbs.v
@@ -1,0 +1,28 @@
+From HTTP2.src Require Import HPACK.HPACKTypes Util.OptionE.
+Require Import String BinNat.
+From ExtLib Require Import Monad MonadExc.
+
+Module Type HPACK.
+  Parameter encodeHeader : DTable -> HeaderList -> string.
+
+  Definition Err := sum HPACKError.
+
+  Parameter decodeHeader : string -> Monad Err -> MonadExc HPACKError Err
+                           -> Err HeaderList.
+
+  Definition defaultDTableSize : N := 4096.
+
+  Parameter newDTable : N -> DTable.
+
+  Inductive CompressionAlgo :=
+  | Naive : CompressionAlgo (* No compression *)
+  | Static : CompressionAlgo (* Using indices in the static table only *)
+  | Linear : CompressionAlgo (* Using indices *).
+
+  Inductive EncodeStrategy :=
+  | encodeStrategy : CompressionAlgo (* Which compression algorithm is used. *)
+                     -> bool (* Whether or not to use Huffman encoding for strings. *)
+                     -> EncodeStrategy.
+
+  Definition defaultEncodeStrategy : EncodeStrategy := encodeStrategy Linear false.
+End HPACK.
